Expand SemQuot example a bit

Pdl/SemQuot.lean
@@ -5,11 +5,13 @@ import Pdl.Semantics
 
 #print semEquiv
 
-theorem semEquiv.Equivalence : Equivalence semEquiv :=
-  ⟨ by convert semEquiv.refl
+def semEquiv.Equivalence : Equivalence semEquiv :=
+  ⟨semEquiv.refl
   , by convert semEquiv.symm
   , by convert semEquiv.trans ⟩
   -- (why) are the "by convert" needed here?
+  -- not for refl, seems it's an autoimplicit issue
+  -- probably because `Equivalence` is in core, whereas `Symmetric`, and `Transitive` are in Mathlib.
 
 instance Formula.instSetoid : Setoid Formula := ⟨semEquiv, semEquiv.Equivalence⟩
 
@@ -18,8 +20,40 @@ abbrev SemProp := Quotient Formula.instSetoid
 
 -- Now, can we lift connectives such as ~ and ⋀ to the quotient?
 
+lemma Formula.neg_congr {φ ψ : Formula} (h : φ ≈ ψ) : Formula.neg φ ≈ Formula.neg ψ :=
+  by simp [HasEquiv.Equiv, Setoid.r, semEquiv] at *
+     intros W M w
+     simp_all only
+
+lemma Formula.and_congr {φ₁ ψ₁ φ₂ ψ₂ : Formula} (h₁ : φ₁ ≈ φ₂) (h₂ : ψ₁ ≈ ψ₂) :
+  Formula.and φ₁ ψ₁ ≈ Formula.and φ₂ ψ₂ :=
+  by simp [HasEquiv.Equiv, Setoid.r, semEquiv] at *
+     intros W M w
+     simp_all only
+
+-- This should maybe go in mathlib? or it exists there somewhere?
+lemma congr_liftFun {α β : Type} [Setoid α] [Setoid β] {f : α → β}
+ (h : ∀ x y, x ≈ y → f x ≈ f y) : ((· ≈ ·) ⇒ (· ≈ ·)) f f :=
+ -- by exact? -- does not work (it's not there at least so obviously)
+  by intro x y hxy; exact h x y hxy
+
+lemma congr_liftFun₂ {α β : Type} [Setoid α] [Setoid β] [Setoid γ] {f : α → β → γ}
+ (h : ∀ (x₁ x₂ : α) (y₁ y₂ : β), x₁ ≈ x₂ → y₁ ≈ y₂ → f x₁ y₁ ≈ f x₂ y₂) :
+ ((· ≈ ·) ⇒ (· ≈ ·) ⇒ (· ≈ ·)) f f :=
+  by intro x₁ x₂ hx y₁ y₂ hy; exact h x₁ x₂ y₁ y₂ hx hy
+
+
 def SemProp.neg : SemProp → SemProp :=
-  Quotient.map Formula.neg (by sorry)
+  Quotient.map Formula.neg (by apply congr_liftFun; apply Formula.neg_congr)
 
 def SemProp.and : SemProp → SemProp → SemProp :=
-  Quotient.map₂ Formula.and (by sorry)
+  Quotient.map₂ Formula.and (by apply congr_liftFun₂; intros x₁ x₂ y₁ y₂ hx hy; exact Formula.and_congr hx hy)
+
+example {φ ψ : Formula} (h : φ ≈ ψ) : Quotient.mk Formula.instSetoid φ = Quotient.mk _ ψ :=
+  by apply Quotient.sound; exact h
+
+example {φ ψ : Formula} (h : φ ≈ ψ) : Quotient.mk Formula.instSetoid (Formula.neg φ) = Quotient.mk _ (Formula.neg ψ) :=
+  by apply Quotient.sound; apply Formula.neg_congr; exact h
+
+example {φ ψ : Formula} (h : φ ≈ ψ) : SemProp.neg (Quotient.mk Formula.instSetoid φ) = SemProp.neg (Quotient.mk _ ψ) :=
+  by apply Quotient.sound; apply Formula.neg_congr; exact h -- why does this work without using neg?
